Add a structure for the proof

arm/proofs/aes_xts_decrypt.ml
@@ -779,11 +779,74 @@ let AESDEC_TAC =
   AP_THM_TAC THEN AP_TERM_TAC THEN
   GEN_REWRITE_TAC LAND_CONV [WORD_XOR_SYM] THEN REFL_TAC;;
 
+let TWEAK_UPDATE_CONV =
+  let ADD_SUC_1 = ARITH_RULE `!n. n + 1 = SUC(n)` in
+  let ADD_SUC_2 = ARITH_RULE `!n. n + 2 = SUC(n + 1)` in
+  let ADD_SUC_3 = ARITH_RULE `!n. n + 3 = SUC(n + 2)` in
+  let ADD_SUC_4 = ARITH_RULE `!n. n + 4 = SUC(n + 3)` in
+  let ADD_SUC_5 = ARITH_RULE `!n. n + 5 = SUC(n + 4)` in
+  let ADD_SUC_6 = ARITH_RULE `!n. n + 6 = SUC(n + 5)` in
+  let ADD_SUC_7 = ARITH_RULE `!n. n + 7 = SUC(n + 6)` in
+  let ADD_SUC_8 = ARITH_RULE `!n. n + 8 = SUC(n + 7)` in
+  let ADD_SUC_9 = ARITH_RULE `!n. n + 9 = SUC(n + 8)` in
+  NUM_REDUCE_CONV THENC
+  RATOR_CONV (LAND_CONV (num_CONV ORELSEC
+    FIRST_CONV
+    [ CHANGED_CONV (ONCE_REWRITE_CONV [ADD_SUC_1]);
+      CHANGED_CONV (ONCE_REWRITE_CONV [ADD_SUC_2]);
+      CHANGED_CONV (ONCE_REWRITE_CONV [ADD_SUC_3]);
+      CHANGED_CONV (ONCE_REWRITE_CONV [ADD_SUC_4]);
+      CHANGED_CONV (ONCE_REWRITE_CONV [ADD_SUC_5]);
+      CHANGED_CONV (ONCE_REWRITE_CONV [ADD_SUC_6]);
+      CHANGED_CONV (ONCE_REWRITE_CONV [ADD_SUC_7]);
+      CHANGED_CONV (ONCE_REWRITE_CONV [ADD_SUC_8]);
+      CHANGED_CONV (ONCE_REWRITE_CONV [ADD_SUC_9]);])) THENC
+  REWRITE_CONV [CONJUNCT2 calculate_tweak] THENC
+  GF_128_MULT_BY_PRIMITIVE_CONV;;
+
+let TWEAK_TAC reg ind indm1 =
+  let lower_term = subst [ind,`ind:num`] `(word_zx:int128->int64) (calculate_tweak ind iv key2)` in
+  let upper_term = subst [ind,`ind:num`] `(word_subword:int128->num#num->int64) (calculate_tweak ind iv key2) (64,64)` in
+  let full_term = subst [ind,`ind:num`] `calculate_tweak ind iv key2` in
+  let full_lemma = subst [reg,`reg:(armstate,int128)component`] `read (reg:(armstate,int128)component) (s:armstate) = a ==> !a'. a = a' ==> read reg s = a'` in
+  let abbrev_term = subst [indm1,`indm1:num`] `tweak_pre:int128 = (calculate_tweak indm1 iv key2)` in
+  FIRST_X_ASSUM(MP_TAC o SPEC lower_term
+    o  MATCH_MP (MESON[] `read X9 s = a ==> !a'. a = a' ==> read X9 s = a'`)) THEN
+    ANTS_TAC THENL [CONV_TAC (RAND_CONV (RAND_CONV TWEAK_UPDATE_CONV)) THEN
+      ABBREV_TAC abbrev_term THEN
+      BITBLAST_TAC; DISCH_TAC] THEN
+  FIRST_X_ASSUM(MP_TAC o SPEC upper_term
+    o  MATCH_MP (MESON[] `read X10 s = a ==> !a'. a = a' ==> read X10 s = a'`)) THEN
+    ANTS_TAC THENL [CONV_TAC (RAND_CONV (RATOR_CONV (RAND_CONV TWEAK_UPDATE_CONV))) THEN
+      ABBREV_TAC abbrev_term THEN
+      BITBLAST_TAC; DISCH_TAC] THEN
+  FIRST_X_ASSUM(MP_TAC o SPEC full_term
+    o  MATCH_MP (MESON[] full_lemma)) THEN
+    ANTS_TAC THENL [CONV_TAC (RAND_CONV TWEAK_UPDATE_CONV) THEN
+      ABBREV_TAC abbrev_term THEN
+      BITBLAST_TAC; DISCH_TAC];;
+
+let XTSDEC_TAC reg ind ind_tweak =
+  let tm = subst [ind, `ind:num`; ind_tweak, `ind_tweak:num`]
+            `aes256_xts_decrypt_round (bytes_to_int128 (SUB_LIST (ind,0x10) (ct:byte list)))
+              (calculate_tweak ind_tweak iv key2) key1` in
+  let lemma = subst [reg, `reg:(armstate,int128)component`]
+            `read (reg:(armstate,int128)component) (s:armstate) = a ==> !a'. a = a' ==> read reg s = a'` in
+  let _ = print_term tm in
+  let _ = print_term lemma in
+  FIRST_X_ASSUM(MP_TAC o SPEC tm o  MATCH_MP (MESON[] lemma)) THEN
+      ANTS_TAC THENL
+      [ EXPAND_TAC "key1" THEN
+        CONV_TAC (RAND_CONV (
+          REWRITE_CONV [aes256_xts_decrypt_round] THENC
+          DEPTH_CONV let_CONV)) THEN
+        AESDEC_TAC; DISCH_TAC ];;
+
 (** Proof **)
 
-let AES_XTS_DECRYPT_CORRECT = prove(
+let AES_XTS_DECRYPT_1BLOCK_CORRECT = prove(
   `!ct_ptr pt_ptr key0_ptr key1_ptr iv_ptr ib iv
-    k00 k01 k02 k03 k04 k05 k06 k07 k08 k09 k0a k0b k0c k0d k0e
+    (k00:int128) k01 k02 k03 k04 k05 k06 k07 k08 k09 k0a k0b k0c k0d k0e
     k10 k11 k12 k13 k14 k15 k16 k17 k18 k19 k1a k1b k1c k1d k1e
     pc.
     nonoverlapping (word pc, LENGTH aes_xts_decrypt_mc) (pt_ptr, 16)
@@ -837,4 +900,798 @@ let AES_XTS_DECRYPT_CORRECT = prove(
     (* Simulate to the end *)
     ARM_ACCSTEPS_TAC AES_XTS_DECRYPT_EXEC [] (127--137) THEN
     ENSURES_FINAL_STATE_TAC THEN ASM_REWRITE_TAC []
+);;
+
+
+(*******************************************)
+(* Full proof *)
+
+(* Taken from Amanda's code at https://github.com/amanda-zx/s2n-bignum/blob/ed25519/arm/sha512/utils.ml *)
+
+let byte_list_at = define
+  `byte_list_at (m : byte list) (m_p : int64) s =
+    ! i. i < LENGTH m ==> read (memory :> bytes8(word_add m_p (word i))) s = EL i m`;;
+
+let tail_len_lt_16_lemma = prove(
+  `!tail_len:int64.
+    word_and len (word 0xf) = tail_len ==> val tail_len < 16`,
+  BITBLAST_TAC
+);;
+
+let num_blocks_ge_80_lemma = prove(
+  `!num_blocks:int64.
+    word_and len (word 0xfffffffffffffff0) = num_blocks /\ val len >= 0x50
+    ==> val num_blocks >= 0x50`,
+  BITBLAST_TAC
+);;
+
+let crock_lemma = prove(
+  `!a:num b:num. a >= b /\ b > 0 ==> ~(a DIV b = 0)`,
+  REPEAT GEN_TAC THEN
+  MP_TAC (SPECL [`a:num`; `b:num`] DIV_EQ_0) THEN
+  ARITH_TAC
+);;
+
+let word_split_lemma = prove(
+  `!len:int64. len = word_add (word_and len (word 0xf))
+                              (word_and len (word 0xfffffffffffffff0))`,
+  BITBLAST_TAC);;
+
+let blt_lemma = prove(
+  `!len:int64 x:num.
+    val len >= x /\ val len < 2 EXP 63
+    ==> (ival (word_sub len (word x)) < &0 <=> ~(ival len - &x = ival (word_sub len (word x))))`,
+  REPEAT STRIP_TAC THEN
+  CHEAT_TAC);;
+
+let UDIV_OPT_LEMMA = prove(
+  `!n:int64. val n < 2 EXP 64 ==>
+    word_ushr
+      ((word ((val (word_and n (word 0xfffffffffffffff0)) * 0xcccccccccccccccd) DIV 0x2 EXP 0x40)):int64)
+      0x6 = word ((val n) DIV 0x50)`,
+  REPEAT STRIP_TAC THEN
+  CHEAT_TAC);;
+
+let READ_CT_LEMMA = prove(
+  `!ct_ptr s ct i.
+    (forall j.
+          j < LENGTH ct
+          ==> read (memory :> bytes8 (word_add ct_ptr (word j))) s = EL j ct)
+          /\ ~(LENGTH ct < 0x50)
+          /\ i < LENGTH ct DIV 0x50  ==>
+    read (memory :> bytes128 (word_add ct_ptr (word_mul (word 0x50) (word i)))) s0 =
+      bytes_to_int128 (SUB_LIST (i * 80, 16) ct) /\
+    read (memory :> bytes128 (word_add (word_add ct_ptr (word_mul (word 0x50) (word i))) (word 0x10))) s =
+      bytes_to_int128 (SUB_LIST (i * 80 + 16, 16) ct) /\
+    read (memory :> bytes128 (word_add (word_add ct_ptr (word_mul (word 0x50) (word i))) (word 0x20))) s =
+      bytes_to_int128 (SUB_LIST (i * 80 + 32, 16) ct) /\
+    read (memory :> bytes128 (word_add (word_add ct_ptr (word_mul (word 0x50) (word i))) (word 0x30))) s =
+      bytes_to_int128 (SUB_LIST (i * 80 + 48, 16) ct) /\
+    read (memory :> bytes128 (word_add (word_add ct_ptr (word_mul (word 0x50) (word i))) (word 0x40))) s =
+      bytes_to_int128 (SUB_LIST (i * 80 + 64, 16) ct)
+    `,
+  CHEAT_TAC
+);;
+
+let READ_CT_TAIL4_LEMMA = prove(
+  `!ct_ptr s ct len (num_blocks:int64) (num_5blocks_adjusted:int64).
+    (forall j.
+          j < LENGTH ct
+          ==> read (memory :> bytes8 (word_add ct_ptr (word j))) s = EL j ct)
+          /\ ~(LENGTH ct < 0x50)
+          /\ val len = LENGTH ct
+          /\ word_and len (word 0xfffffffffffffff0) = num_blocks
+          /\ val
+      (word_sub
+       (word_sub (num_blocks_adjusted:int64)
+       (word_mul (word 0x50) num_5blocks_adjusted))
+      (word 0x40)) =
+      0x0
+    ==>
+    read (memory :> bytes128 (word_add
+      (word_add ct_ptr (word_mul (word 0x50) num_5blocks_adjusted))
+      (word 0x30))) s =
+      bytes_to_int128 (SUB_LIST (val num_5blocks_adjusted * 16 + 0x30, 16) ct) /\
+    read (memory :> bytes128 (word_add
+      (word_add ct_ptr (word_mul (word 0x50) num_5blocks_adjusted))
+      (word 0x20))) s =
+      bytes_to_int128 (SUB_LIST (val num_5blocks_adjusted * 16 + 0x20, 16) ct) /\
+    read (memory :> bytes128 (word_add
+      (word_add ct_ptr (word_mul (word 0x50) num_5blocks_adjusted))
+      (word 0x10))) s =
+      bytes_to_int128 (SUB_LIST (val num_5blocks_adjusted * 16 + 0x10, 16) ct) /\
+    read (memory :> bytes128
+      (word_add ct_ptr (word_mul (word 0x50) num_5blocks_adjusted))) s =
+      bytes_to_int128 (SUB_LIST (val num_5blocks_adjusted * 16, 16) ct)
+    `,
+  CHEAT_TAC
+);;
+
+let READ_CT_TAIL3_LEMMA = prove(
+  `!ct_ptr s ct len (num_blocks:int64) (num_5blocks_adjusted:int64).
+    (forall j.
+          j < LENGTH ct
+          ==> read (memory :> bytes8 (word_add ct_ptr (word j))) s = EL j ct)
+          /\ ~(LENGTH ct < 0x50)
+          /\ val len = LENGTH ct
+          /\ word_and len (word 0xfffffffffffffff0) = num_blocks
+          /\ val
+      (word_sub
+       (word_sub (num_blocks_adjusted:int64)
+       (word_mul (word 0x50) num_5blocks_adjusted))
+      (word 0x30)) =
+      0x0
+    ==>
+    read (memory :> bytes128 (word_add
+      (word_add ct_ptr (word_mul (word 0x50) num_5blocks_adjusted))
+      (word 0x20))) s =
+      bytes_to_int128 (SUB_LIST (val num_5blocks_adjusted * 16 + 0x20, 16) ct) /\
+    read (memory :> bytes128 (word_add
+      (word_add ct_ptr (word_mul (word 0x50) num_5blocks_adjusted))
+      (word 0x10))) s =
+      bytes_to_int128 (SUB_LIST (val num_5blocks_adjusted * 16 + 0x10, 16) ct) /\
+    read (memory :> bytes128
+      (word_add ct_ptr (word_mul (word 0x50) num_5blocks_adjusted))) s =
+      bytes_to_int128 (SUB_LIST (val num_5blocks_adjusted * 16, 16) ct)
+    `,
+  CHEAT_TAC
+);;
+
+let READ_CT_TAIL2_LEMMA = prove(
+  `!ct_ptr s ct len (num_blocks:int64) (num_5blocks_adjusted:int64).
+    (forall j.
+          j < LENGTH ct
+          ==> read (memory :> bytes8 (word_add ct_ptr (word j))) s = EL j ct)
+          /\ ~(LENGTH ct < 0x50)
+          /\ val len = LENGTH ct
+          /\ word_and len (word 0xfffffffffffffff0) = num_blocks
+          /\ val
+      (word_sub
+       (word_sub num_blocks_adjusted
+       (word_mul (word 0x50) num_5blocks_adjusted))
+      (word 0x20)) =
+      0x0
+    ==>
+    read (memory :> bytes128 (word_add
+      (word_add ct_ptr (word_mul (word 0x50) num_5blocks_adjusted))
+      (word 0x10))) s =
+      bytes_to_int128 (SUB_LIST (val num_5blocks_adjusted * 16 + 0x10, 16) ct) /\
+    read (memory :> bytes128
+      (word_add ct_ptr (word_mul (word 0x50) num_5blocks_adjusted))) s =
+      bytes_to_int128 (SUB_LIST (val num_5blocks_adjusted * 16, 16) ct)
+    `,
+  CHEAT_TAC
+);;
+
+let READ_CT_TAIL1_LEMMA = prove(
+  `!ct_ptr s ct len (num_blocks:int64) (num_5blocks_adjusted:int64).
+    (forall j.
+          j < LENGTH ct
+          ==> read (memory :> bytes8 (word_add ct_ptr (word j))) s = EL j ct)
+          /\ ~(LENGTH ct < 0x50)
+          /\ val len = LENGTH ct
+          /\ word_and len (word 0xfffffffffffffff0) = num_blocks
+          /\ val
+      (word_sub
+       (word_sub num_blocks_adjusted
+       (word_mul (word 0x50) num_5blocks_adjusted))
+      (word 0x10)) =
+      0x0
+    ==>
+    read (memory :> bytes128
+      (word_add ct_ptr (word_mul (word 0x50) num_5blocks_adjusted))) s =
+      bytes_to_int128 (SUB_LIST (val num_5blocks_adjusted * 16, 16) ct)
+    `,
+  CHEAT_TAC
+);;
+
+let AES_XTS_DECRYPT_CORRECT = prove(
+  `!ct_ptr pt_ptr ct pt_init key1_ptr key2_ptr iv_ptr iv len
+    k00 k01 k02 k03 k04 k05 k06 k07 k08 k09 k0a k0b k0c k0d k0e
+    k10 k11 k12 k13 k14 k15 k16 k17 k18 k19 k1a k1b k1c k1d k1e
+    pc.
+    nonoverlapping (word pc, LENGTH aes_xts_decrypt_mc) (pt_ptr, val len)
+    /\ val len >= 16 /\ val len <= 2 EXP 24 /\ val len = LENGTH ct
+    ==> ensures arm
+    (\s. aligned_bytes_loaded s (word pc) aes_xts_decrypt_mc /\
+         read PC s = word (pc + 0x1c) /\
+         C_ARGUMENTS [ct_ptr; pt_ptr; len; key1_ptr; key2_ptr; iv_ptr] s /\
+         byte_list_at ct ct_ptr s /\
+         byte_list_at pt_init pt_ptr s /\
+         read(memory :> bytes128 iv_ptr) s = iv /\
+         set_key_schedule s key1_ptr k00 k01 k02 k03 k04 k05 k06 k07 k08 k09 k0a k0b k0c k0d k0e /\
+         set_key_schedule s key2_ptr k10 k11 k12 k13 k14 k15 k16 k17 k18 k19 k1a k1b k1c k1d k1e)
+    (\s. read PC s = word (pc + 0xb00) /\
+         byte_list_at (aes256_xts_decrypt ct (val len) iv
+              [k00; k01; k02; k03; k04; k05; k06; k07; k08; k09; k0a; k0b; k0c; k0d; k0e]
+              [k10; k11; k12; k13; k14; k15; k16; k17; k18; k19; k1a; k1b; k1c; k1d; k1e]
+              pt_init) pt_ptr s
+         )
+    (MAYCHANGE [PC] ,, MAYCHANGE [events] ,,
+     MAYCHANGE [X21;X2;X6;X4;X9;X10;X19;X22;X11;X7;X0;X1;X8] ,,
+     MAYCHANGE [Q6;Q1;Q0;Q8;Q9;Q10;Q11;Q16;Q17;Q12;Q13;Q14;Q15;
+                Q4;Q5;Q18;Q19;Q20;Q21;Q22;Q23;Q7;Q29;Q24;Q25;Q26] ,,
+     MAYCHANGE SOME_FLAGS,, MAYCHANGE [memory :> bytes(pt_ptr, val len)])
+    `,
+    REWRITE_TAC [(REWRITE_CONV [aes_xts_decrypt_mc] THENC LENGTH_CONV) `LENGTH aes_xts_decrypt_mc`] THEN
+    REWRITE_TAC[set_key_schedule; C_ARGUMENTS; SOME_FLAGS; NONOVERLAPPING_CLAUSES; byte_list_at] THEN
+    REPEAT STRIP_TAC THEN
+
+    (* Break len into full blocks and tail *)
+    SUBGOAL_THEN `len:int64 = word_add (word_and len (word 0xf))
+      (word_and len (word 0xfffffffffffffff0))` ASSUME_TAC THENL
+    [REWRITE_TAC[word_split_lemma]; ALL_TAC] THEN
+    ABBREV_TAC `num_blocks:int64 = word_and len (word 0xfffffffffffffff0)` THEN
+    ABBREV_TAC `tail_len:int64 = word_and len (word 0xf)` THEN
+    ABBREV_TAC `key1:int128 list = [k00; k01; k02; k03; k04; k05; k06; k07; k08; k09; k0a; k0b; k0c; k0d; k0e]` THEN
+    ABBREV_TAC `key2:int128 list = [k10; k11; k12; k13; k14; k15; k16; k17; k18; k19; k1a; k1b; k1c; k1d; k1e]` THEN
+
+    (* Case splits on length:
+      len < 16 -- error case
+      len < 32 -- one block, or one block and a tail
+      len < 48 -- two blocks, or two blocks and a tail
+      len < 64 -- three blocks, or three blocks and a tail
+      len < 80 -- four blocks, or four blocks and a tail
+      len < 96 -- five blocks, or five blocks and a tail
+      len >= 96 -- six blocks and up
+
+      Note: for decrypt, because of cipherstealing, there needs to be one extra
+      block at the end together with the tail to be processed for cipherstealing
+     *)
+    ASM_CASES_TAC `val (len:int64) < 96` THENL [CHEAT_TAC; ALL_TAC] THEN
+
+    ABBREV_TAC `num_blocks_adjusted = if val (tail_len:int64) = 0
+          then num_blocks else word_sub (num_blocks:int64) (word 0x10)` THEN
+    ABBREV_TAC `num_5blocks_adjusted = (word (val (num_blocks_adjusted:int64) DIV 0x50)):int64` THEN
+
+    (* Verify properties of the program until the beginning of the loop.
+       The properties include the invariant, and a bunch of other initial setup.
+     *)
+    ENSURES_SEQUENCE_TAC `pc + 0x170`
+    `\s.
+        read X0 s = ct_ptr /\
+        read X1 s = pt_ptr /\
+        read X2 s = num_blocks_adjusted /\
+        read X3 s = key1_ptr /\
+        read X21 s = tail_len /\
+        read X8 s = num_5blocks_adjusted /\
+        read Q6 s = calculate_tweak 0 iv key2 /\
+        read Q8 s = calculate_tweak 1 iv key2 /\
+        read Q9 s = calculate_tweak 2 iv key2 /\
+        read Q10 s = calculate_tweak 3 iv key2 /\
+        read Q11 s = calculate_tweak 4 iv key2 /\
+        read X19 s = word 0x87 /\
+        read X10 s = word_subword (calculate_tweak 4 iv key2) (64,64) /\
+        read X9 s = word_zx (calculate_tweak 4 iv key2) /\
+        read Q16 s = k00 /\ read Q17 s = k01 /\ read Q12 s = k02 /\ read Q13 s = k03 /\
+        read Q14 s = k04 /\ read Q15 s = k05 /\ read Q4 s = k06 /\ read Q5 s = k07 /\
+        read Q18 s = k08 /\ read Q19 s = k09 /\ read Q20 s = k0a /\ read Q21 s = k0b /\
+        read Q22 s = k0c /\ read Q23 s = k0d /\ read Q7 s = k0e /\
+        byte_list_at ct ct_ptr s /\
+        byte_list_at (aes256_xts_decrypt ct 0 iv key1 key2 pt_init) pt_ptr s /\
+        set_key_schedule s key1_ptr k00 k01 k02 k03 k04 k05 k06 k07 k08 k09 k0a k0b k0c k0d k0e` THEN
+        CONJ_TAC THENL
+        [
+          (* ===> Symbolic Simulation: Start symbolic simulation*)
+          ENSURES_INIT_TAC "s0" THEN
+          ARM_ACCSTEPS_TAC AES_XTS_DECRYPT_EXEC [] (1--2) THEN
+          (* Discharge if condition *)
+          SUBGOAL_THEN
+            `ival (word_sub (word_add (tail_len:int64) (num_blocks:int64)) (word 0x10)) < &0x0 <=>
+          ~(ival (word_add tail_len num_blocks) - &0x10 =
+            ival (word_sub (word_add tail_len num_blocks) (word 0x10)))` ASSUME_TAC THENL
+          [ MATCH_MP_TAC blt_lemma THEN CONJ_TAC THENL
+            [ UNDISCH_TAC `len:int64 = word_add tail_len num_blocks` THEN
+              UNDISCH_TAC `val (len:int64) >= 16` THEN
+              WORD_ARITH_TAC;
+              UNDISCH_TAC `len:int64 = word_add tail_len num_blocks` THEN
+              UNDISCH_TAC `val (len:int64) <= 2 EXP 24` THEN
+              WORD_ARITH_TAC];
+            ALL_TAC] THEN
+          POP_ASSUM(fun th -> RULE_ASSUM_TAC(REWRITE_RULE[th])) THEN
+
+          (* ===> Symbolic Simulation: Symbolic execution for initialization of tweak *)
+          ARM_ACCSTEPS_TAC AES_XTS_DECRYPT_EXEC [] (3--69) THEN
+          (* Prove Q6 stores initial tweak *)
+          FIRST_X_ASSUM(MP_TAC o SPEC `(calculate_tweak 0 iv key2)`
+            o  MATCH_MP (MESON[] `read Q6 s = a ==> !a'. a = a' ==> read Q6 s = a'`)) THEN
+          ANTS_TAC THENL
+          [REWRITE_TAC[CONJUNCT1 calculate_tweak; xts_init_tweak] THEN
+           EXPAND_TAC "key2" THEN AESENC_TAC; DISCH_TAC] THEN
+
+          (* ===> Symbolic Simulation: Symbolic simulating untill next branch *)
+          ARM_ACCSTEPS_TAC AES_XTS_DECRYPT_EXEC [] (70--89) THEN
+          (* Case split on whether there is a tail *)
+          FIRST_X_ASSUM MP_TAC THEN
+          COND_CASES_TAC THENL
+          [
+            (* If there is no tail *)
+            DISCH_TAC THEN
+            (* Prove x9, x10 stores lower and upper halves and Q8 stores the full tweak *)
+            TWEAK_TAC `Q8:(armstate,int128)component` `1:num` `0:num` THEN
+            ARM_ACCSTEPS_TAC AES_XTS_DECRYPT_EXEC [] (90--93) THEN
+            (* Prove the optimized udiv is basically udiv *)
+            SUBGOAL_THEN `word_ushr ((word ((val (word_and (word_add (tail_len:int64) num_blocks)
+              (word 0xfffffffffffffff0)) * 0xcccccccccccccccd) DIV 0x2 EXP 0x40)):int64)
+              0x6 = word ((val num_blocks) DIV 0x50)` ASSUME_TAC THENL
+            [ CHEAT_TAC
+             ; ALL_TAC] THEN
+            POP_ASSUM(fun th -> RULE_ASSUM_TAC(REWRITE_RULE[th])) THEN
+
+            (* Eliminate 1 block case *)
+            ARM_ACCSTEPS_TAC AES_XTS_DECRYPT_EXEC [] (94--95) THEN
+            SUBGOAL_THEN `~(val (word_and (word_add (tail_len:int64) num_blocks) (word 0xfffffffffffffff0)) < 0x20)` ASSUME_TAC THENL
+            [CHEAT_TAC; POP_ASSUM(fun th -> RULE_ASSUM_TAC(REWRITE_RULE[th]))] THEN
+            (* Eliminate 2 blocks case *)
+            ARM_ACCSTEPS_TAC AES_XTS_DECRYPT_EXEC [] (96--97) THEN
+            SUBGOAL_THEN `~(val (word_and (word_add (tail_len:int64) num_blocks) (word 0xfffffffffffffff0)) < 0x30)` ASSUME_TAC THENL
+            [CHEAT_TAC; POP_ASSUM(fun th -> RULE_ASSUM_TAC(REWRITE_RULE[th]))] THEN
+            (* Eliminate 3 blocks case and prove Q9 stores tweak 2 *)
+            ARM_ACCSTEPS_TAC AES_XTS_DECRYPT_EXEC [] (98--105) THEN
+            SUBGOAL_THEN `~(val (word_and (word_add (tail_len:int64) num_blocks) (word 0xfffffffffffffff0)) < 0x40)` ASSUME_TAC THENL
+            [CHEAT_TAC; POP_ASSUM(fun th -> RULE_ASSUM_TAC(REWRITE_RULE[th]))] THEN
+            TWEAK_TAC `Q9:(armstate,int128)component` `2:num` `1:num` THEN
+
+            (* Eliminate 4 blocks case and Q10 stores tweak 3 *)
+            ARM_ACCSTEPS_TAC AES_XTS_DECRYPT_EXEC [] (106--113) THEN
+            SUBGOAL_THEN `~(val (word_and (word_add (tail_len:int64) num_blocks) (word 0xfffffffffffffff0)) < 0x50)` ASSUME_TAC THENL
+            [CHEAT_TAC; POP_ASSUM(fun th -> RULE_ASSUM_TAC(REWRITE_RULE[th]))] THEN
+            TWEAK_TAC `Q10:(armstate,int128)component` `3:num` `2:num` THEN
+
+            (* Must have 5 blocks, execute until start of loop. Q11 stores tweak 4 *)
+            ARM_ACCSTEPS_TAC AES_XTS_DECRYPT_EXEC [] (114--122) THEN
+            TWEAK_TAC `Q11:(armstate,int128)component` `4:num` `3:num` THEN
+
+            ENSURES_FINAL_STATE_TAC THEN ASM_REWRITE_TAC[] THEN
+            REPEAT CONJ_TAC THENL
+            [
+              CHEAT_TAC;
+              REWRITE_TAC[SYM (ASSUME `len:int64 = word_add tail_len num_blocks`)] THEN
+              ASM_REWRITE_TAC[];
+              CHEAT_TAC;
+              ASM_REWRITE_TAC[byte_list_at];
+              CHEAT_TAC;
+              ASM_REWRITE_TAC[set_key_schedule]]
+            ; ALL_TAC
+          ] THEN
+
+          (* If there is a tail *)
+          DISCH_TAC THEN
+          ARM_ACCSTEPS_TAC AES_XTS_DECRYPT_EXEC [] (90--92) THEN
+          (* Discharge if condition *)
+          SUBGOAL_THEN
+            `ival
+            (word_sub
+             (word_sub
+              (word_and (word_add (tail_len:int64) num_blocks)
+              (word 0xfffffffffffffff0))
+             (word 0x10))
+            (word 0x10)) <
+            &0x0 <=>
+            ~(ival
+              (word_sub
+               (word_and (word_add tail_len num_blocks)
+               (word 0xfffffffffffffff0))
+              (word 0x10)) -
+              &0x10 =
+              ival
+              (word_sub
+               (word_sub
+                (word_and (word_add tail_len num_blocks)
+                (word 0xfffffffffffffff0))
+               (word 0x10))
+              (word 0x10)))` ASSUME_TAC THENL
+          [ CHEAT_TAC;
+            ALL_TAC] THEN
+          POP_ASSUM(fun th -> RULE_ASSUM_TAC(REWRITE_RULE[th])) THEN
+
+          (* Prove x9, x10 stores lower and upper halves and Q8 stores the full tweak *)
+          TWEAK_TAC `Q8:(armstate,int128)component` `1:num` `0:num` THEN
+          ARM_ACCSTEPS_TAC AES_XTS_DECRYPT_EXEC [] (93--96) THEN
+          (* Prove the optimized udiv is basically udiv *)
+          SUBGOAL_THEN `word_ushr
+      (word
+      ((val
+        (word_sub
+         (word_and (word_add (tail_len:int64) num_blocks) (word 0xfffffffffffffff0))
+        (word 0x10)) *
+        0xcccccccccccccccd) DIV
+       0x2 EXP 0x40):int64)
+      0x6 = word ((val (word_sub num_blocks (word 1))) DIV 0x50)` ASSUME_TAC THENL
+          [ CHEAT_TAC
+            ; ALL_TAC] THEN
+          POP_ASSUM(fun th -> RULE_ASSUM_TAC(REWRITE_RULE[th])) THEN
+
+          (* Eliminate 1 block case *)
+          ARM_ACCSTEPS_TAC AES_XTS_DECRYPT_EXEC [] (97--98) THEN
+          SUBGOAL_THEN `~(val
+          (word_sub
+           (word_and (word_add (tail_len:int64) num_blocks)
+           (word 0xfffffffffffffff0))
+          (word 0x10)) <
+          0x20)` ASSUME_TAC THENL
+          [CHEAT_TAC; POP_ASSUM(fun th -> RULE_ASSUM_TAC(REWRITE_RULE[th]))] THEN
+          (* Eliminate 2 blocks case *)
+          ARM_ACCSTEPS_TAC AES_XTS_DECRYPT_EXEC [] (99--100) THEN
+          SUBGOAL_THEN `~(val
+          (word_sub
+           (word_and (word_add (tail_len:int64) num_blocks)
+           (word 0xfffffffffffffff0))
+          (word 0x10)) <
+          0x30)` ASSUME_TAC THENL
+          [CHEAT_TAC; POP_ASSUM(fun th -> RULE_ASSUM_TAC(REWRITE_RULE[th]))] THEN
+          (* Eliminate 3 blocks case and prove Q9 stores tweak 2 *)
+          ARM_ACCSTEPS_TAC AES_XTS_DECRYPT_EXEC [] (101--108) THEN
+          SUBGOAL_THEN `~(val
+          (word_sub
+           (word_and (word_add (tail_len:int64) num_blocks)
+           (word 0xfffffffffffffff0))
+          (word 0x10)) <
+          0x40)` ASSUME_TAC THENL
+          [CHEAT_TAC; POP_ASSUM(fun th -> RULE_ASSUM_TAC(REWRITE_RULE[th]))] THEN
+          TWEAK_TAC `Q9:(armstate,int128)component` `2:num` `1:num` THEN
+
+          (* Eliminate 4 blocks case and Q10 stores tweak 3 *)
+          ARM_ACCSTEPS_TAC AES_XTS_DECRYPT_EXEC [] (109--116) THEN
+          SUBGOAL_THEN `~(val
+          (word_sub
+           (word_and (word_add (tail_len:int64) num_blocks)
+           (word 0xfffffffffffffff0))
+          (word 0x10)) <
+          0x50)` ASSUME_TAC THENL
+          [CHEAT_TAC; POP_ASSUM(fun th -> RULE_ASSUM_TAC(REWRITE_RULE[th]))] THEN
+          TWEAK_TAC `Q10:(armstate,int128)component` `3:num` `2:num` THEN
+
+          (* Must have 5 blocks, execute until start of loop. Q11 stores tweak 4 *)
+          ARM_ACCSTEPS_TAC AES_XTS_DECRYPT_EXEC [] (117--125) THEN
+          TWEAK_TAC `Q11:(armstate,int128)component` `4:num` `3:num` THEN
+
+          ENSURES_FINAL_STATE_TAC THEN ASM_REWRITE_TAC[] THEN
+          REPEAT CONJ_TAC THENL
+          [
+            CHEAT_TAC;
+            REWRITE_TAC[SYM (ASSUME `len:int64 = word_add tail_len num_blocks`)] THEN
+            ASM_REWRITE_TAC[];
+            CHEAT_TAC;
+            ASM_REWRITE_TAC[byte_list_at];
+            CHEAT_TAC;
+            ASM_REWRITE_TAC[set_key_schedule]]
+          ; ALL_TAC
+        ] THEN
+
+    (* Prove the rest of the program *)
+    (* Setting up the loop invariant *)
+
+    (* Invariant:
+      X0 holds ct_ptr + i*0x50
+      X1 hols pt_ptr + i*0x50
+      X3 holds key1_ptr
+      X21 holds tail_len
+
+      X2 holds number of blocks left
+      X8 holds number of 5xblocks left
+      Q6, Q8, Q9, Q10, Q11 holds the next 5 tweaks
+      X10 stores upper half of last tweak
+      X9 stores lower half of last tweak
+      X19 holds 0x87
+      Q16, Q17, Q12, Q13, Q14, Q15, Q4, Q5, Q18, Q19, Q20, Q21, Q22, Q23, Q7 stores the key1
+      Memory: ct_ptr points to the input data blocks
+      Memory: Up to the new five blocks in output pt_ptr matche the specification
+    *)
+
+    ENSURES_WHILE_PAUP_TAC
+      `0`
+      `val (num_5blocks_adjusted:int64)`
+      `pc + 0x170`
+      `pc + 0x460`
+      `\i s.
+        (read X0 s = word_add ct_ptr (word_mul (word 0x50) (word i)) /\
+         read X1 s = word_add pt_ptr (word_mul (word 0x50) (word i)) /\
+         read X3 s = key1_ptr /\
+         read X21 s = tail_len /\
+         read X2 s = word_sub num_blocks_adjusted (word_mul (word 0x50) (word i)) /\
+         read X8 s = word_sub num_5blocks_adjusted (word i) /\
+         read Q6 s = calculate_tweak (i * 5) iv key2 /\
+         read Q8 s = calculate_tweak (i * 5 + 1) iv key2 /\
+         read Q9 s = calculate_tweak (i * 5 + 2) iv key2 /\
+         read Q10 s = calculate_tweak (i * 5 + 3) iv key2 /\
+         read Q11 s = calculate_tweak (i * 5 + 4) iv key2 /\
+         read X19 s = word 0x87 /\
+         read X10 s = word_subword (calculate_tweak (i * 5 + 4) iv key2) (64,64) /\
+         read X9 s = word_zx (calculate_tweak (i * 5 + 4) iv key2) /\
+         read Q16 s = k00 /\ read Q17 s = k01 /\ read Q12 s = k02 /\ read Q13 s = k03 /\
+         read Q14 s = k04 /\ read Q15 s = k05 /\ read Q4 s = k06 /\ read Q5 s = k07 /\
+         read Q18 s = k08 /\ read Q19 s = k09 /\ read Q20 s = k0a /\ read Q21 s = k0b /\
+         read Q22 s = k0c /\ read Q23 s = k0d /\ read Q7 s = k0e /\
+         byte_list_at ct ct_ptr s /\
+         byte_list_at (aes256_xts_decrypt ct (i * 5 * 16) iv key1 key2 pt_init) pt_ptr s) /\
+        // loop backedge condition
+        (read ZF s <=> i = val (num_5blocks_adjusted:int64))` THEN
+    ASM_REWRITE_TAC[] THEN REPEAT CONJ_TAC THENL
+    [
+      (* Subgoal 1. Bound of loop is not zero *)
+      CHEAT_TAC;
+
+      (* Subgoal 2. Invariant holds before entering the loop *)
+      REWRITE_TAC[byte_list_at] THEN
+      ENSURES_INIT_TAC "s0" THEN
+      ENSURES_FINAL_STATE_TAC THEN ASM_REWRITE_TAC[] THEN
+      REPEAT CONJ_TAC THENL
+      [
+        WORD_ARITH_TAC; WORD_ARITH_TAC;
+        CHEAT_TAC;
+        CHEAT_TAC;
+        CONV_TAC NUM_REDUCE_CONV;
+        CONV_TAC NUM_REDUCE_CONV;
+        CONV_TAC NUM_REDUCE_CONV;
+        CONV_TAC NUM_REDUCE_CONV;
+        CONV_TAC NUM_REDUCE_CONV;
+        CONV_TAC NUM_REDUCE_CONV;
+        CONV_TAC NUM_REDUCE_CONV;
+        CONV_TAC NUM_REDUCE_CONV THEN ASM_REWRITE_TAC[byte_list_at]
+      ];
+
+      (* Subgoal 3: loop body *)
+      REPEAT STRIP_TAC THEN
+      (* ===> Symbolic Simulation: Start symbolic simulation*)
+      REWRITE_TAC[byte_list_at] THEN
+      SUBGOAL_THEN `i < LENGTH (ct:byte list) DIV 0x50` ASSUME_TAC THENL
+      [CHEAT_TAC;ALL_TAC] THEN
+      SUBGOAL_THEN `~(LENGTH (ct:byte list) < 0x50)` ASSUME_TAC THENL
+      [CHEAT_TAC;ALL_TAC] THEN
+
+      GHOST_INTRO_TAC `b0:int128` `read (memory :> bytes128 (word_add pt_ptr (word_mul (word 0x50) (word i))))` THEN
+      GHOST_INTRO_TAC `b1:int128` `read (memory :> bytes128 (word_add (word_add pt_ptr (word_mul (word 0x50) (word i))) (word 0x10)))` THEN
+      GHOST_INTRO_TAC `b2:int128` `read (memory :> bytes128 (word_add (word_add pt_ptr (word_mul (word 0x50) (word i))) (word 0x20)))` THEN
+      GHOST_INTRO_TAC `b3:int128` `read (memory :> bytes128 (word_add (word_add pt_ptr (word_mul (word 0x50) (word i))) (word 0x30)))` THEN
+      GHOST_INTRO_TAC `b4:int128` `read (memory :> bytes128 (word_add (word_add pt_ptr (word_mul (word 0x50) (word i))) (word 0x40)))` THEN
+
+      ENSURES_INIT_TAC "s0" THEN
+      (* List values for ct_ptr + [0 .. 0x40] *)
+      MP_TAC (SPECL [`ct_ptr:int64`; `s0:armstate`; `ct:byte list`; `i:num`] READ_CT_LEMMA) THEN
+      ASM_REWRITE_TAC[] THEN REPEAT STRIP_TAC THEN
+      ARM_ACCSTEPS_TAC AES_XTS_DECRYPT_EXEC [] (1--151) THEN
+      (* Prove Q0, Q1, Q24, Q25, Q26 stores correct plaintext *)
+      (* and prove Q6, Q8, Q9, Q10, Q11 stores correct tweak *)
+      XTSDEC_TAC `Q0:(armstate,int128)component` `i * 0x50` `i * 0x5` THEN
+      TWEAK_TAC `Q6:(armstate,int128)component` `i * 5 + 5` `i * 5 + 4` THEN
+
+      ARM_ACCSTEPS_TAC AES_XTS_DECRYPT_EXEC [] (152--159) THEN
+      XTSDEC_TAC `Q1:(armstate,int128)component` `i * 0x50 + 0x10` `i * 0x5 + 0x1` THEN
+      TWEAK_TAC `Q8:(armstate,int128)component` `i * 5 + 6` `i * 5 + 5` THEN
+
+      ARM_ACCSTEPS_TAC AES_XTS_DECRYPT_EXEC [] (160--167) THEN
+      XTSDEC_TAC `Q24:(armstate,int128)component` `i * 0x50 + 0x20` `i * 0x5 + 0x2` THEN
+      TWEAK_TAC `Q9:(armstate,int128)component` `i * 5 + 7` `i * 5 + 6` THEN
+
+      ARM_ACCSTEPS_TAC AES_XTS_DECRYPT_EXEC [] (168--175) THEN
+      XTSDEC_TAC `Q25:(armstate,int128)component` `i * 0x50 + 0x30` `i * 0x5 + 0x3` THEN
+      TWEAK_TAC `Q10:(armstate,int128)component` `i * 5 + 8` `i * 5 + 7` THEN
+
+      ARM_ACCSTEPS_TAC AES_XTS_DECRYPT_EXEC [] (176--183) THEN
+      XTSDEC_TAC `Q26:(armstate,int128)component` `i * 0x50 + 0x40` `i * 0x5 + 0x4` THEN
+      TWEAK_TAC `Q11:(armstate,int128)component` `i * 5 + 9` `i * 5 + 8` THEN
+
+      (* Simulate until end of loop *)
+      ARM_ACCSTEPS_TAC AES_XTS_DECRYPT_EXEC [] (184--188) THEN
+      ENSURES_FINAL_STATE_TAC THEN ASM_REWRITE_TAC[] THEN
+      REPEAT CONJ_TAC THENL
+      [ CHEAT_TAC;
+        CHEAT_TAC;
+        CHEAT_TAC;
+        CHEAT_TAC;
+        CHEAT_TAC;
+        CHEAT_TAC;
+        CHEAT_TAC;
+        CHEAT_TAC;
+        CHEAT_TAC;
+        CHEAT_TAC;
+        CHEAT_TAC;
+        CHEAT_TAC;
+        CHEAT_TAC;
+        CHEAT_TAC;
+        CHEAT_TAC
+      ];
+
+
+      (* Subgoal 4: prove backedge is taken if i != val num_5blocks_adjusted *)
+      REPEAT STRIP_TAC THEN
+      REWRITE_TAC[byte_list_at] THEN
+      ENSURES_INIT_TAC "s0" THEN
+      ARM_ACCSTEPS_TAC AES_XTS_DECRYPT_EXEC [] (1--1) THEN
+      SUBGOAL_THEN `~(val (word_sub (num_5blocks_adjusted:int64) (word i)) = 0x0)` ASSUME_TAC THENL
+      [CHEAT_TAC; ALL_TAC] THEN
+      POP_ASSUM(fun th -> RULE_ASSUM_TAC(REWRITE_RULE[th])) THEN
+      ENSURES_FINAL_STATE_TAC THEN ASM_REWRITE_TAC[];
+
+
+      (* Subgoal 5: Prove the invariant implies post-condition
+                    Backedge instruction is executed here *)
+      REPEAT STRIP_TAC THEN
+      REWRITE_TAC[byte_list_at] THEN
+      SUBGOAL_THEN `~(LENGTH (ct:byte list) < 0x50)` ASSUME_TAC THENL
+      [CHEAT_TAC;ALL_TAC] THEN
+      SUBGOAL_THEN `(word (val (num_5blocks_adjusted:int64))):int64 = num_5blocks_adjusted` SUBST_ALL_TAC THENL
+      [CHEAT_TAC;ALL_TAC] THEN
+
+      GHOST_INTRO_TAC `bt_0:int128`
+        `read (memory :> bytes128 (word_add pt_ptr (word_mul (word 0x50) (num_5blocks_adjusted:int64))))` THEN
+      GHOST_INTRO_TAC `bt_1:int128`
+        `read (memory :> bytes128 (word_add (word_add pt_ptr (word_mul (word 0x50) (num_5blocks_adjusted:int64))) (word 0x10)))` THEN
+      GHOST_INTRO_TAC `bt_2:int128`
+        `read (memory :> bytes128 (word_add (word_add (pt_ptr:int64) (word_mul (word 0x50) (num_5blocks_adjusted:int64))) (word 0x20)))` THEN
+      GHOST_INTRO_TAC `bt_3:int128`
+        `read (memory :> bytes128 (word_add (word_add (pt_ptr:int64) (word_mul (word 0x50) (num_5blocks_adjusted:int64))) (word 0x30)))` THEN
+
+      ENSURES_INIT_TAC "s0" THEN
+      ARM_ACCSTEPS_TAC AES_XTS_DECRYPT_EXEC [] (1--3) THEN
+      FIRST_X_ASSUM MP_TAC THEN
+
+      COND_CASES_TAC THENL
+      [ (* Case: len % 0x50 = 0x40 *)
+        DISCH_TAC THEN
+
+        MP_TAC (SPECL [`ct_ptr:int64`; `s3:armstate`; `ct:byte list`;
+          `len:int64`; `num_blocks:int64`; `num_5blocks_adjusted:int64`] READ_CT_TAIL4_LEMMA) THEN
+        ASM_REWRITE_TAC[] THEN REPEAT STRIP_TAC THEN
+
+        ARM_ACCSTEPS_TAC AES_XTS_DECRYPT_EXEC [] (4--125) THEN
+        XTSDEC_TAC `Q0:(armstate,int128)component`
+          `val (num_5blocks_adjusted:int64) * 0x10` `val (num_5blocks_adjusted:int64) * 0x5` THEN
+        XTSDEC_TAC `Q1:(armstate,int128)component`
+          `val (num_5blocks_adjusted:int64) * 0x10 + 0x10` `val (num_5blocks_adjusted:int64) * 0x5 + 0x1` THEN
+        XTSDEC_TAC `Q24:(armstate,int128)component`
+          `val (num_5blocks_adjusted:int64) * 0x10 + 0x20` `val (num_5blocks_adjusted:int64) * 0x5 + 0x2` THEN
+        XTSDEC_TAC `Q25:(armstate,int128)component`
+          `val (num_5blocks_adjusted:int64) * 0x10 + 0x30` `val (num_5blocks_adjusted:int64) * 0x5 + 0x3` THEN
+
+        ARM_ACCSTEPS_TAC AES_XTS_DECRYPT_EXEC [] (126--133) THEN
+        TWEAK_TAC `Q6:(armstate,int128)component` `val (num_5blocks_adjusted:int64) * 0x5 + 0x4` `val (num_5blocks_adjusted:int64) * 0x5 + 0x3` THEN
+
+        (* The following lemmas are for NONSELFMODIFYING_STATE_UPDATE_TAC when store back to pt_ptr *)
+        RULE_ASSUM_TAC(REWRITE_RULE
+          [WORD_RULE `word_mul (word 0x50) num_5blocks_adjusted:int64 = word(0x50 * val num_5blocks_adjusted)`]) THEN
+        SUBGOAL_THEN `80 * val(num_5blocks_adjusted:int64) + 64 <= val(len:int64)`
+          ASSUME_TAC THENL [CHEAT_TAC; ALL_TAC] THEN
+
+        ARM_ACCSTEPS_TAC AES_XTS_DECRYPT_EXEC [] (134--138) THEN
+        FIRST_X_ASSUM MP_TAC THEN
+        COND_CASES_TAC THENL
+        [
+          DISCH_TAC THEN
+          ENSURES_FINAL_STATE_TAC THEN ASM_REWRITE_TAC[] THEN
+          CHEAT_TAC;
+          ALL_TAC
+        ] THEN
+        (* Cipher stealing branch *)
+        CHEAT_TAC;
+        ALL_TAC
+      ] THEN
+
+      DISCH_TAC THEN
+      ARM_ACCSTEPS_TAC AES_XTS_DECRYPT_EXEC [] (4--5) THEN
+      FIRST_X_ASSUM MP_TAC THEN
+      COND_CASES_TAC THENL
+      [ (* Case: len % 0x50 = 0x30 *)
+        DISCH_TAC THEN
+        MP_TAC (SPECL [`ct_ptr:int64`; `s5:armstate`; `ct:byte list`; `len:int64`; `num_blocks:int64`; `num_5blocks_adjusted:int64`] READ_CT_TAIL3_LEMMA) THEN
+        ASM_REWRITE_TAC[] THEN REPEAT STRIP_TAC THEN
+
+        ARM_ACCSTEPS_TAC AES_XTS_DECRYPT_EXEC [] (6--97) THEN
+        XTSDEC_TAC `Q0:(armstate,int128)component`
+          `val (num_5blocks_adjusted:int64) * 0x10` `val (num_5blocks_adjusted:int64) * 0x5` THEN
+        XTSDEC_TAC `Q1:(armstate,int128)component`
+          `val (num_5blocks_adjusted:int64) * 0x10 + 0x10` `val (num_5blocks_adjusted:int64) * 0x5 + 0x1` THEN
+        XTSDEC_TAC `Q24:(armstate,int128)component`
+          `val (num_5blocks_adjusted:int64) * 0x10 + 0x20` `val (num_5blocks_adjusted:int64) * 0x5 + 0x2` THEN
+
+        ARM_ACCSTEPS_TAC AES_XTS_DECRYPT_EXEC [] (98--105) THEN
+        TWEAK_TAC `Q6:(armstate,int128)component` `val (num_5blocks_adjusted:int64) * 0x5 + 0x3` `val (num_5blocks_adjusted:int64) * 0x5 + 0x2` THEN
+
+        (* The following lemmas are for NONSELFMODIFYING_STATE_UPDATE_TAC when store back to pt_ptr *)
+        RULE_ASSUM_TAC(REWRITE_RULE
+          [WORD_RULE `word_mul (word 0x50) num_5blocks_adjusted:int64 = word(0x50 * val num_5blocks_adjusted)`]) THEN
+        SUBGOAL_THEN `80 * val(num_5blocks_adjusted:int64) + 48 <= val(len:int64)`
+          ASSUME_TAC THENL [CHEAT_TAC; ALL_TAC] THEN
+
+        ARM_ACCSTEPS_TAC AES_XTS_DECRYPT_EXEC [] (106--110) THEN
+        FIRST_X_ASSUM MP_TAC THEN
+        COND_CASES_TAC THENL
+        [
+          DISCH_TAC THEN
+          ENSURES_FINAL_STATE_TAC THEN ASM_REWRITE_TAC[] THEN
+          CHEAT_TAC;
+          ALL_TAC
+        ] THEN
+        (* Cipher stealing branch *)
+        CHEAT_TAC;
+        ALL_TAC
+      ] THEN
+
+      DISCH_TAC THEN
+      ARM_ACCSTEPS_TAC AES_XTS_DECRYPT_EXEC [] (6--7) THEN
+      FIRST_X_ASSUM MP_TAC THEN
+      COND_CASES_TAC THENL
+      [ (* Case: len % 0x50 = 0x20 *)
+        DISCH_TAC THEN
+        MP_TAC (SPECL [`ct_ptr:int64`; `s7:armstate`; `ct:byte list`; `len:int64`; `num_blocks:int64`; `num_5blocks_adjusted:int64`] READ_CT_TAIL2_LEMMA) THEN
+        ASM_REWRITE_TAC[] THEN REPEAT STRIP_TAC THEN
+
+        ARM_ACCSTEPS_TAC AES_XTS_DECRYPT_EXEC [] (8--68) THEN
+        XTSDEC_TAC `Q0:(armstate,int128)component`
+          `val (num_5blocks_adjusted:int64) * 0x10` `val (num_5blocks_adjusted:int64) * 0x5` THEN
+        XTSDEC_TAC `Q1:(armstate,int128)component`
+          `val (num_5blocks_adjusted:int64) * 0x10 + 0x10` `val (num_5blocks_adjusted:int64) * 0x5 + 0x1` THEN
+
+        (* The following lemmas are for NONSELFMODIFYING_STATE_UPDATE_TAC when store back to pt_ptr *)
+        RULE_ASSUM_TAC(REWRITE_RULE
+          [WORD_RULE `word_mul (word 0x50) num_5blocks_adjusted:int64 = word(0x50 * val num_5blocks_adjusted)`]) THEN
+        SUBGOAL_THEN `80 * val(num_5blocks_adjusted:int64) + 32 <= val(len:int64)`
+          ASSUME_TAC THENL [CHEAT_TAC; ALL_TAC] THEN
+
+        ARM_ACCSTEPS_TAC AES_XTS_DECRYPT_EXEC [] (69--77) THEN
+        TWEAK_TAC `Q6:(armstate,int128)component` `val (num_5blocks_adjusted:int64) * 0x5 + 0x2` `val (num_5blocks_adjusted:int64) * 0x5 + 0x1` THEN
+
+        ARM_ACCSTEPS_TAC AES_XTS_DECRYPT_EXEC [] (78--80) THEN
+        FIRST_X_ASSUM MP_TAC THEN
+        COND_CASES_TAC THENL
+        [
+          DISCH_TAC THEN
+          ENSURES_FINAL_STATE_TAC THEN ASM_REWRITE_TAC[] THEN
+          CHEAT_TAC;
+          ALL_TAC
+        ] THEN
+        (* Cipher stealing branch *)
+        CHEAT_TAC;
+        ALL_TAC] THEN
+
+      DISCH_TAC THEN
+      ARM_ACCSTEPS_TAC AES_XTS_DECRYPT_EXEC [] (8--9) THEN
+      FIRST_X_ASSUM MP_TAC THEN
+      COND_CASES_TAC THENL
+      [ (* Case: len % 0x50 = 0x10 *)
+        DISCH_TAC THEN
+        MP_TAC (SPECL [`ct_ptr:int64`; `s9:armstate`; `ct:byte list`; `len:int64`; `num_blocks:int64`; `num_5blocks_adjusted:int64`] READ_CT_TAIL1_LEMMA) THEN
+        ASM_REWRITE_TAC[] THEN REPEAT STRIP_TAC THEN
+
+        ARM_ACCSTEPS_TAC AES_XTS_DECRYPT_EXEC [] (10--40) THEN
+        XTSDEC_TAC `Q0:(armstate,int128)component`
+          `val (num_5blocks_adjusted:int64) * 0x10` `val (num_5blocks_adjusted:int64) * 0x5` THEN
+
+        (* The following lemmas are for NONSELFMODIFYING_STATE_UPDATE_TAC when store back to pt_ptr *)
+        RULE_ASSUM_TAC(REWRITE_RULE
+          [WORD_RULE `word_mul (word 0x50) num_5blocks_adjusted:int64 = word(0x50 * val num_5blocks_adjusted)`]) THEN
+        SUBGOAL_THEN `80 * val(num_5blocks_adjusted:int64) + 16 <= val(len:int64)`
+          ASSUME_TAC THENL [CHEAT_TAC; ALL_TAC] THEN
+
+        ARM_ACCSTEPS_TAC AES_XTS_DECRYPT_EXEC [] (41--49) THEN
+        TWEAK_TAC `Q6:(armstate,int128)component` `val (num_5blocks_adjusted:int64) * 0x5 + 0x1` `val (num_5blocks_adjusted:int64) * 0x5` THEN
+
+        ARM_ACCSTEPS_TAC AES_XTS_DECRYPT_EXEC [] (50--52) THEN
+        FIRST_X_ASSUM MP_TAC THEN
+        COND_CASES_TAC THENL
+        [
+          DISCH_TAC THEN
+          ENSURES_FINAL_STATE_TAC THEN ASM_REWRITE_TAC[] THEN
+          CHEAT_TAC;
+          ALL_TAC
+        ] THEN
+        (* Cipher stealing branch *)
+        CHEAT_TAC;
+        ALL_TAC] THEN
+
+      (* Case: len % 0x50 = 0 *)
+      DISCH_TAC THEN
+      ARM_ACCSTEPS_TAC AES_XTS_DECRYPT_EXEC [] (10--12) THEN
+      FIRST_X_ASSUM MP_TAC THEN
+      COND_CASES_TAC THENL
+      [
+        DISCH_TAC THEN
+        ENSURES_FINAL_STATE_TAC THEN ASM_REWRITE_TAC[] THEN
+        CHEAT_TAC;
+        ALL_TAC
+      ] THEN
+      (* Cipher stealing branch *)
+      CHEAT_TAC
+    ]
 );;
