arm/proofs/aes_xts_decrypt_spec.ml
@@ -172,9 +172,13 @@ let aes256_xts_decrypt = new_definition
         APPEND (FST res) Ptail`;;
 
 (*******************************************)
-(* Test vectors *)
+(* Test vectors printed from AWS-LC *)
 
 (*
+The decrypt key schedule is different from encrypt.
+This is because AWS-LC uses EQINVCIPHER() for AES decryption.
+See 5.3.5 EQINVCIPHER() from NIST.FIPS.197 Advanced Encryption Standard (AES)
+
 key1:
 c70a951e84370d1836bdd387607e94e5
 7ead95d6f74bf6b3103340cce21b473d
@@ -564,6 +568,7 @@ time (REWRITE_CONV [iv_tweak;KEY1;KEY2;perror] THENC AES256_XTS_DECRYPT_CONV)
 (*******************************************)
 (* Tests *)
 
+(*
 (* 1 block : 81 second *)
 time prove (`aes256_xts_decrypt c0 16 iv_tweak KEY1 KEY2 perror = p0`,
   CONV_TAC(LAND_CONV (REWRITE_CONV [c0;iv_tweak;KEY1;KEY2;perror] THENC AES256_XTS_DECRYPT_CONV)) THEN
@@ -574,7 +579,8 @@ time prove(`aes256_xts_decrypt c1 22 iv_tweak KEY1 KEY2 perror = p1`,
   CONV_TAC(LAND_CONV (REWRITE_CONV [c1;iv_tweak;KEY1;KEY2;perror;p1] THENC AES256_XTS_DECRYPT_CONV)) THEN
   REWRITE_TAC [p1] THEN REFL_TAC);;
 
-(* 3 blocks + 3 bytes : 206 seconds *)
+(* 3 blocks + 3 bytes : 273 seconds *)
 time prove(`aes256_xts_decrypt c2 51 iv_tweak KEY1 KEY2 perror = p2`,
   CONV_TAC(LAND_CONV (REWRITE_CONV [c2;iv_tweak;KEY1;KEY2;perror;p2] THENC AES256_XTS_DECRYPT_CONV)) THEN
   REWRITE_TAC [p2] THEN REFL_TAC);;
+*)
